proofs/oracle.mli
@@ -1,0 +1,91 @@
+
+type bool =
+| True
+| False
+
+type nat =
+| O
+| S of nat
+
+type 'a option =
+| Some of 'a
+| None
+
+type ('a, 'b) prod =
+| Pair of 'a * 'b
+
+val fst : ('a1, 'a2) prod -> 'a1
+
+val snd : ('a1, 'a2) prod -> 'a2
+
+type 'a list =
+| Nil
+| Cons of 'a * 'a list
+
+val app : 'a1 list -> 'a1 list -> 'a1 list
+
+type comparison =
+| Eq
+| Lt
+| Gt
+
+module Nat :
+ sig
+  val eqb : nat -> nat -> bool
+
+  val compare : nat -> nat -> comparison
+ end
+
+val map : ('a1 -> 'a2) -> 'a1 list -> 'a2 list
+
+val flat_map : ('a1 -> 'a2 list) -> 'a1 list -> 'a2 list
+
+val fold_right : ('a2 -> 'a1 -> 'a1) -> 'a1 -> 'a2 list -> 'a1
+
+type proc =
+| Zero
+| Inp of name * proc
+| Lift of name * proc
+| Drop of name
+| Par of proc * proc
+and name =
+| Var of nat
+| Quote of proc
+
+val proc_compare : proc -> proc -> comparison
+
+val name_compare : name -> name -> comparison
+
+val pleb : proc -> proc -> bool
+
+val flatten_par : proc -> proc list
+
+val insert_proc : proc -> proc list -> proc list
+
+val sort_par : proc list -> proc list
+
+val rebuild : proc list -> proc
+
+val norm_par : proc -> proc
+
+val canon : proc -> proc
+
+val canon_name : name -> name
+
+val proc_beq : proc -> proc -> bool
+
+val name_beq : name -> name -> bool
+
+val subst_name : name -> nat -> name -> name
+
+val subst_sem : proc -> nat -> name -> proc
+
+val sync : name -> name -> bool
+
+val selects : proc list -> (proc, proc list) prod list
+
+val comm_reduct : proc -> proc -> proc list -> proc option
+
+val redexes : proc list -> proc list
+
+val step : proc -> proc list
